ulib/FStar.Util.fst
@@ -7,5 +7,5 @@ let op_Hat_Plus_Hat  x y = (TSet.singleton x) ++ (TSet.singleton y)
 open FStar.Heap
 open FStar.HyperHeap
 let op_At_Plus_At (#a:Type) (#r:rid) (#b:Type) (#s:rid) (x:rref r a) (y:rref s b) =
-   Ref (as_ref x) ^+^ Ref (as_ref y)
-let op_Plus_Plus_At (#a:Type) (#r:rid) (x:TSet.set aref) (y:rref r a) = x ++^ Ref (as_ref y)
+   Set.union (Set.singleton (addr_of (as_ref x))) (Set.singleton (addr_of (as_ref y)))
+let op_Plus_Plus_At (#a:Type) (#r:rid) (x:Set.set nat) (y:rref r a) = Set.union x (Set.singleton (addr_of (as_ref y)))
